lift tactic: almost works

src/Pipit.Sugar.Shallow.Tactics.Lift.fst
@@ -17,13 +17,18 @@
 
   Manually inserting these primitives isn't too bad for small programs, but
   it gets noisy in large programs. Pipit has two additional complexities that
-  make it even noisier. First, streams are restricted to store "statically-bounded"
-  types, so that we can generate good statically-allocated C code. To support
-  this, we use a slightly different form of lifted applications that lets us
-  distinguish between partially-applied functions and real streams. The second
-  complexity is that we want to annotate each primitive with some unique
-  identifier, so that a later common-subexpression-elimination pass can check
-  whether two operations are equal.
+  make it even noisier.
+
+  First, streams are restricted to store "statically-bounded" types, which in
+  our case outlaws streams of functions. Unfortunately, the intermediate stream
+  `(+) <$> element` has type `stream (int -> int)`,
+  which we do not support as a runtime type. To work around this, we use a
+  separate type for intermediate applications; this application type is
+  restricted and can't be delayed or stored in stream variables.
+
+  The second complexity is that we want to annotate each primitive with some
+  unique identifier, so that a later common-subexpression-elimination pass can
+  check whether two operations are equal. This is currently unimplemented.
 
   High-level question:
     * is this a massive hack? Should this use the new DSL framework instead?
@@ -31,17 +36,26 @@
   Implementation questions / limitations:
     * record constructors and record field accessors do not typecheck with FStar.Tactics.tc
     * mutual recursion isn't exposed by Tac.inspect. Exposing this would be a big change, wouldn't it?
-    * any way to give error locations in Tac.fail?
 *)
 module Pipit.Sugar.Shallow.Tactics.Lift
 
 module Ref = FStar.Reflection.V2
 module Tac = FStar.Tactics.V2
 
+module TermEq = FStar.Reflection.V2.TermEq
+
+module Range = FStar.Range
+
 module List = FStar.List.Tot
 
-// #push-options "--print_implicits --print_full_names --ugly"
+#push-options "--print_implicits --print_full_names --ugly --print_bound_var_types"
 
+let fail (#a: Type) (msg: string) (rng: Range.range) (ctx: list string): Tac.Tac a =
+  let str0 = "Lift transform: failure at " ^ Tac.range_to_string rng ^ "\n  " ^ msg in
+  let str = List.fold_left (fun str str' -> str ^ "\n    * " ^ str') str0 ctx in
+  Tac.fail str
+
+let range_of_term' (tm: Tac.term): Range.range = Ref.range_of_term tm
 
 let rec zip2 (#x #y: Type) (xs: list x) (ys: list y): list (x & y)
   = match xs, ys with
@@ -74,6 +88,10 @@ assume val liftP'apply (#a: eqtype) (#ft: Type) (f: stream_app (a -> ft)) (ea: s
 
 assume val liftP'close (#a: eqtype) (ea: stream_app a): stream a
 
+
+// assume val liftP'close_lemma (#p: prop) (f: stream_app (squash p)): stream unit
+// assume val liftP'apply_lemma (#a: eqtype) (#ft: a -> prop) (f: stream_app ((xa: a) -> Lemma (ft a))) (ea: stream a): stream_app (ft a)
+
 assume val rec' (#a: eqtype) (f: stream a -> stream a): stream a
 
 assume val (let^) (#a #b: eqtype) (f: stream a) (g: stream a -> stream b): stream b
@@ -83,7 +101,6 @@ let stream'name: Tac.name = ["Pipit"; "Sugar"; "Shallow"; "Tactics"; "Lift"; "st
 let static'name: Tac.name = ["Pipit"; "Sugar"; "Shallow"; "Tactics"; "Lift"; "static"]
 let as_static'name: Tac.name = ["Pipit"; "Sugar"; "Shallow"; "Tactics"; "Lift"; "as_static"]
 
-// TODO: argument qualifier implicit/explicit in ModeFun
 type mode = | Stream | Static | ModeFun: mode -> explicit: bool -> mode -> mode
 
 let debug_print str = Tac.print str
@@ -97,15 +114,27 @@ let env_push (b: Tac.binder) (m: mode) (e: env): env =
   { tac_env  = Ref.push_namedv e.tac_env (Ref.pack_namedv b);
     mode_env = (b.uniq, m) :: e.mode_env }
 
-let env_get_mode (b: Tac.namedv) (e: env): Tac.Tac mode =
+let env_get_mode (b: Tac.namedv) (e: env) (rng: Range.range): Tac.Tac mode =
   match List.find (fun (uniq,m) -> uniq = b.uniq) e.mode_env with
-  | None -> Tac.fail ("no such binder: b" ^ Tac.namedv_to_string b)
+  | None ->
+    fail ("no such binder: b" ^ Tac.namedv_to_string b)
+      rng []
   | Some (_, m) -> m
 
-let assert_type_annotation (ty: Tac.term) (err: string): Tac.Tac unit =
+let rec env_push_pat (p: Tac.pattern) (m: mode) (e: env): Tac.Tac env =
+  match p with
+  | Tac.Pat_Constant _ -> e
+  | Tac.Pat_Cons c ->
+    Tac.fold_left (fun e (p,_) -> env_push_pat p m e) e c.subpats
+  | Tac.Pat_Var v ->
+    env_push (Tac.namedv_to_binder v.v (Tac.unseal v.sort)) m e
+  | Tac.Pat_Dot_Term _ -> e
+
+
+let assert_type_annotation (ty: Tac.term) (rng: Range.range) (ctx: list string): Tac.Tac unit =
   match Tac.inspect_unascribe ty with
   | Tac.Tv_Unknown ->
-    Tac.fail ("Lift.descend: error: requires explicit type annotation: " ^ err)
+    fail "error: term requires explicit type annotation" rng ctx
   | _ -> ()
 
 let qual_is_explicit (q: Ref.aqualv): bool =
@@ -124,15 +153,20 @@ let rec mode_of_ty (ty: Tac.term): Tac.Tac mode =
       // then Some Static
       else Static
     | _ -> Static)
-  | Tac.Tv_Arrow arg (Tac.C_Total res) ->
+  | Tac.Tv_Arrow arg (Tac.C_Total res)
+  | Tac.Tv_Arrow arg (Tac.C_GTotal res)
+  // We don't support general effects, but parse them anyway in case the effect is Tot
+  | Tac.Tv_Arrow arg (Tac.C_Eff _ _ res _ _) ->
     ModeFun (mode_of_ty arg.sort) (qual_is_explicit arg.qual) (mode_of_ty res)
+  | Tac.Tv_Arrow arg (Tac.C_Lemma _ _ _) ->
+    ModeFun (mode_of_ty arg.sort) (qual_is_explicit arg.qual) Static
   | _ -> Static
 
-let mode_join (m1 m2: mode): Tac.Tac mode = match m1, m2 with
+let mode_join (rng: Range.range) (m1 m2: mode): Tac.Tac mode = match m1, m2 with
   | Stream, Static -> Stream
   | Static, Stream -> Stream
   | Static, Static -> Static
-  | _, _ -> if m1 = m2 then m1 else Tac.fail ("cannot join incompatible modes: " ^ Tac.term_to_string (quote (m1, m2)))
+  | _, _ -> if m1 = m2 then m1 else fail ("cannot join incompatible modes: " ^ Tac.term_to_string (quote (m1, m2))) rng []
 
 let mode_cast (m_expect: mode) (mt: mode & Tac.term): Tac.Tac (mode & Tac.term) =
   (match mt, m_expect with
@@ -148,28 +182,53 @@ let type_cast (ty: Tac.term) (mt: mode & Tac.term): Tac.Tac (mode & Tac.term) =
     | (Static, tm), Stream -> (Stream, (`return (`#tm)))
     | _ -> mt)
 
-let joins_modes (mts: list (mode & Tac.term)): Tac.Tac (mode & list Tac.term) =
+let joins_modes (rng: Range.range) (mts: list (mode & Tac.term)): Tac.Tac (mode & list Tac.term) =
   match mts with
   | (m0, tm) :: mts' ->
     let ms' = List.map fst mts' in
-    let m = Tac.fold_left mode_join m0 ms' in
+    let m = Tac.fold_left (mode_join rng) m0 ms' in
     (m, Tac.map (fun x -> snd (mode_cast m x)) mts)
   | [] -> (Static, [])
 
-(* get mode of type-annotated function body; requires type annotations *)
+let unwrap_AscribeT (tm: Tac.term): Tac.Tac Tac.term =
+  match Tac.inspect tm with
+  | Tac.Tv_AscribedT tm _ _ _ -> tm
+  | _ -> tm
+
+let lift_stream_match (scrut: Tac.term) (ret: option Tac.match_returns_ascription) (brs: list (Tac.pattern & Tac.term)): Tac.Tac Tac.term =
+  let mk_namedv (pp: string) =
+    { uniq = Tac.fresh (); sort = Tac.seal (`_); ppname = Ref.as_ppname pp } <: Tac.namedv
+  in
+  let nscrut = mk_namedv "scrut" in
+  let nbrs = Tac.map (fun (pat,tm) ->
+    (mk_namedv "branch", pat, tm)) brs in
+  let brs = List.map (fun (nm,pat,tm) -> (pat, Tac.pack (Tac.Tv_Var nm))) nbrs in
+  let xmatch = Tac.pack (Tac.Tv_Match (Tac.pack (Tac.Tv_Var nscrut)) ret brs) in
+  let rec go_abs hd nms: Tac.Tac Tac.term = match nms with
+    | [] -> hd
+    | nm::nms ->
+      go_abs (Tac.pack (Tac.Tv_Abs (Tac.namedv_to_binder nm (`_)) hd)) nms
+  in
+  let rec go_app hd tms: Tac.Tac Tac.term = match tms with
+    | [] -> (`liftP'close (`#hd))
+    | tm::tms ->
+      go_app (`liftP'apply (`#hd) (`#tm)) tms
+  in
+  let abs = go_abs xmatch (List.rev (nscrut :: List.map (fun (nm,_,_) -> nm) nbrs)) in
+  let app = go_app (`liftP'prim (`#abs)) (scrut :: List.map (fun (_,_,tm) -> tm) nbrs) in
+  app
+
+(* get mode of type-annotated function body; requires type annotations
+  This doesn't take an environment as it's used to compute the environment
+  for the letrec subexpressions *)
 let rec mode_of_letrec (t: Tac.term): Tac.Tac mode =
   match Tac.inspect t with
-  // cannot look up in env: as env is not yet known
-  // | Tac.Tv_Var (v: Tac.namedv) ->
-  //   env_get_mode v e
-  // | Tac.Tv_FVar (v: Tac.fv) ->
-  //   mode_of_ty (Tac.tc e.tac_env t)
   | Tac.Tv_Const (vc: Tac.vconst) ->
     Static
 
   | Tac.Tv_Abs bv tm ->
     // abstractions need explicit binders
-    assert_type_annotation bv.sort ("letrec binder " ^ Tac.binder_to_string bv);
+    assert_type_annotation bv.sort (range_of_term' t) ["abstraction " ^ Tac.binder_to_string bv; "in letrec (mode_of_letrec)"];
     let m1 = mode_of_ty bv.sort in
     let m2 = mode_of_letrec tm in
     ModeFun m1 (qual_is_explicit bv.qual) m2
@@ -182,9 +241,12 @@ let rec mode_of_letrec (t: Tac.term): Tac.Tac mode =
     | Tac.C_Total ty | Tac.C_GTotal ty ->
       mode_of_ty ty
     | Tac.C_Lemma _ _ _ -> Static
-    | Tac.C_Eff _ _ _ _ _ -> Tac.fail ("Lift.mode_of_letrec: unsupported effect: " ^ Tac.term_to_string t))
+    | Tac.C_Eff _ _ _ _ _ ->
+      fail ("unsupported effect: " ^ Tac.comp_to_string cmp) (range_of_term' t) ["in letrec (mode_of_letrec)"])
   | _ ->
-    Tac.fail ("Lift.mode_of_letrec: letrecs must have explicit type annotations: " ^ Tac.term_to_string t)
+    fail "letrecs must have explicit type annotations"
+      (range_of_term' t)
+      ["in letrec (mode_of_letrec)"]
 
 let rec descend (e: env) (t: Tac.term): Tac.Tac (mode & Tac.term) =
   let go_stream (e: env) (t: Tac.term) =
@@ -192,13 +254,18 @@ let rec descend (e: env) (t: Tac.term): Tac.Tac (mode & Tac.term) =
     match m with
     | Static -> (`return (`#t))
     | Stream -> t
-    | ModeFun _ _ _ -> Tac.fail ("Lift.descend: cannot lift function to stream: " ^ Tac.term_to_string t)
+    | ModeFun _ _ _ ->
+      fail ("cannot lift function to stream: " ^ Tac.term_to_string t)
+        (range_of_term' t)
+        []
   in
   match Tac.inspect t with
   | Tac.Tv_Var (v: Tac.namedv) ->
-    (env_get_mode v e, t)
+    (env_get_mode v e (range_of_term' t), t)
   | Tac.Tv_BVar (v: Tac.bv) ->
-    Tac.fail ("Lift.descend: unexpected bvar; expected named variables only " ^ Tac.term_to_string t)
+    fail
+      ("unexpected bvar; expected named variables only " ^ Tac.term_to_string t)
+      (range_of_term' t) []
   | Tac.Tv_FVar (v: Tac.fv) ->
     (mode_of_ty (Tac.tc e.tac_env t), t)
   | Tac.Tv_Const (vc: Tac.vconst) ->
@@ -211,7 +278,8 @@ let rec descend (e: env) (t: Tac.term): Tac.Tac (mode & Tac.term) =
 
       | _, (arg,Ref.Q_Meta _) :: _
       | _, (arg,Ref.Q_Implicit) :: _ ->
-        Tac.fail "not supported: cannot lift implicit / meta applications"
+        fail "not supported: cannot lift implicit / meta applications"
+          (range_of_term' arg) ["go_lifts"]
 
       | ModeFun Static _  m2, (arg,_)::args ->
         let (ma, arg) = descend e arg in
@@ -220,7 +288,12 @@ let rec descend (e: env) (t: Tac.term): Tac.Tac (mode & Tac.term) =
 
       | Static, [] -> (Stream, (`liftP'close (`#hd)))
       | _, _ ->
-        Tac.fail ("Lift.descend:go_lifts: cannot lift ! xxxerror bad mode " ^ Tac.term_to_string t)
+        fail ("cannot lift application! bad mode / args")
+          (range_of_term' t)
+            ["mode: " ^ Tac.term_to_string (quote m);
+            "args:"  ^ Tac.term_to_string (quote args);
+            "hd:"  ^ Tac.term_to_string hd;
+            "go_lifts"]
     in
     let rec go_apps m hd args: Tac.Tac (mode & Tac.term) = match m, args with
       | ModeFun _ false m2, (_,Ref.Q_Explicit)::_ ->
@@ -230,14 +303,22 @@ let rec descend (e: env) (t: Tac.term): Tac.Tac (mode & Tac.term) =
         let (ma, arg) = descend e arg in
         (match ma, m1 with
         | Stream, Static ->
-          // TODO assert aq = Explicit; lifted apps only supports explicit
+          (match aq with
+          | Ref.Q_Explicit -> ()
+          | _ ->
+            fail "cannot lift implicit arguments - put all implicit arguments before explicits, or rearrange the arguments with a lambda (TODO)."
+              (range_of_term' arg)
+              ["go_apps"]
+            );
           go_lifts m2 (`liftP'apply (liftP'prim (`#hd)) (`#arg)) args
         | _, _ ->
           let (ma, arg) = mode_cast m1 (ma, arg) in
           go_apps m2 (Tac.pack (Tac.Tv_App hd (arg, aq))) args)
 
-      | _, _ :: _ ->
-        Tac.fail ("Lift.descend:go_apps: too many arguments for mode; " ^ Tac.term_to_string t)
+      | _, (arg,_) :: _ ->
+        fail "too many arguments for mode"
+          (range_of_term' arg)
+          ["go_apps"]
       | _, [] -> (m, hd)
     in
     let (hd, args) = Tac.collect_app t in
@@ -245,15 +326,15 @@ let rec descend (e: env) (t: Tac.term): Tac.Tac (mode & Tac.term) =
     // (as_static x) stops lifting of x, but if the result is applied to
     // another argument, we still want to lift that:
     // > lift ((as_static x) y) ==> x (lift y)
-    if FStar.Reflection.V2.TermEq.term_eq hd (`as_static)
+    if TermEq.term_eq hd (`as_static)
     then match args with
-         | [] -> Tac.fail "impossible"
-         // xxx handle implicit arg
-         | (hd, _)::args -> go_apps (mode_of_ty (Tac.tc e.tac_env hd)) hd args
+         | (hd, Ref.Q_Explicit)::args -> go_apps (mode_of_ty (Tac.tc e.tac_env hd)) hd args
+         | (ty, Ref.Q_Implicit)::(hd, Ref.Q_Explicit)::args -> go_apps (mode_of_ty ty) hd args
+         | _ -> fail "as_static: impossible: expected application" (range_of_term' t) []
     else go_apps mh hd args
   | Tac.Tv_Abs bv tm ->
     // abstractions need explicit binders
-    assert_type_annotation bv.sort (Tac.binder_to_string bv);
+    assert_type_annotation bv.sort (range_of_term' t) ["in abstraction " ^ Tac.binder_to_string bv];
     debug_print ("Abs: descend with " ^ Tac.term_to_string bv.sort);
     let m1 = mode_of_ty bv.sort in
     let (m2, tm) = descend (env_push bv m1 e) tm in
@@ -283,34 +364,60 @@ let rec descend (e: env) (t: Tac.term): Tac.Tac (mode & Tac.term) =
     let (md, def) = descend e def in
     let (md, def) = type_cast b.sort (md,def) in
     let (mb, body) = descend (env_push b md e) body in
-    let bodyabs = Tac.pack (Tac.Tv_Abs b body) in
     let lett = match md, mb with
-      | Stream, Stream -> (`(let^) (`#def) (`#bodyabs))
+      | Stream, Stream ->
+        // HACK: remove unit type annotation from let-bindings: the parser
+        // generates `let x: unit = ... in ...` for semicolons.
+        // we want to lift this to a stream of units, but generally we want
+        // to leave user-written type annotations alone.
+        let b = if TermEq.term_eq b.sort (`unit)
+          then { b with sort = (`stream unit) } <: Tac.simple_binder
+          else b
+        in
+        let bodyabs = Tac.pack (Tac.Tv_Abs b body) in
+        (`(let^) (`#def) (`#bodyabs))
       | _, _ -> Tac.pack (Tac.Tv_Let false attrs b def body)
     in
     (mb, lett)
 
   | Tac.Tv_Match scrut ret brs ->
+    // HACK: remove type ascriptions from match scrutinees: the parser
+    // generates if-expressions with the form `match x <: bool with ...`
+    // but this doesn't work if we lift the scrutinee to a stream.
+    // Maybe we should convert the type ascription to `x <: stream bool`
+    let scrut = unwrap_AscribeT scrut in
     let (ms, scrut) = descend e scrut in
     (match ms with
     | Static ->
-      let mts = Tac.map (fun (pat,tm) -> descend e tm) brs in
-      let (m, ts) = joins_modes mts in
+      debug_print ("match: static scrutinee " ^ Tac.term_to_string scrut);
+      let mts = Tac.map (fun (pat,tm) -> descend (env_push_pat pat Static e) tm) brs in
+      let (mbrs, ts) = joins_modes (range_of_term' t) mts in
       let brs = zip2 (List.map fst brs) ts in
-      (m, Tac.pack (Tac.Tv_Match scrut ret brs))
+      (mbrs, Tac.pack (Tac.Tv_Match scrut ret brs))
     | Stream ->
-      Tac.fail "TODO match"
-      // let rec go_stream brs: Tac.Tac (mode & list Tac.branch) = match brs with
-      //   | [] -> (Static, [])
-      //   | (pat,tm) :: brs ->
-      //     let (m,brs) = go_stream brs in
-      //     let (mt,tm) = descend e tm in
-      //     (mode_join m mt, (pat,tm) :: brs)
-      // in
-      // let (mb, brs) = go_stream brs in
-      // (mb, Tac.pack (Tac.Tv_Match scrut ret brs)))
+      debug_print ("match: stream scrutinee " ^ Tac.term_to_string scrut);
+      // XXX: the current semantics for streaming-matches is more of a "select"
+      // than a match: all of the branches are eagerly evaluated, and then we
+      // just choose which to return based on the scrutinee
+      let rec check_pat p: Tac.Tac unit = match p with
+        | Tac.Pat_Constant _ -> ()
+        | Tac.Pat_Cons c -> Tac.iter (fun (p,_) -> check_pat p) c.subpats
+        | Tac.Pat_Var _ ->
+          fail ("streaming patterns can't bind variables (TODO)")
+            (range_of_term' t) ["in pattern-match"]
+        // not sure what this means...
+        | Tac.Pat_Dot_Term _ -> ()
+      in
+      let check_pat_top p: Tac.Tac unit = match p with
+        // TODO: assert Pat_Var binder is `_` / not mentioned
+        | Tac.Pat_Var _ -> ()
+        | p -> check_pat p
+      in
+      let brs = Tac.map (fun (pat,tm) -> check_pat_top pat; (pat, go_stream e tm)) brs in
+      (Stream, lift_stream_match scrut ret brs)
     | ModeFun _ _ _ ->
-      Tac.fail ("Lift.descend: match scrutinee cannot be function: match " ^ Tac.term_to_string scrut))
+      fail "match scrutinee cannot be function"
+        (range_of_term' scrut) ["in pattern match"])
 
   | Tac.Tv_AscribedT (tm: Tac.term) (ty: Tac.term) tac use_eq ->
     debug_print ("AscribedT: " ^ Tac.term_to_string ty);
@@ -326,7 +433,9 @@ let rec descend (e: env) (t: Tac.term): Tac.Tac (mode & Tac.term) =
       let (mm, tm) = type_cast ty (mm, tm) in
       (mm, Tac.pack (Tac.Tv_AscribedC tm cmp tac use_eq))
       // TODO lemmas etc?
-    | _ -> Tac.fail "unsupported: type ascriptions on effects")
+    | _ ->
+      fail ("unsupported: type ascriptions on effects: " ^ Tac.comp_to_string cmp)
+        (range_of_term' t) [])
 
   // Type stuff: leave alone
   | Tac.Tv_Uvar _ _ -> (Static, t)
@@ -337,7 +446,8 @@ let rec descend (e: env) (t: Tac.term): Tac.Tac (mode & Tac.term) =
   | Tac.Tv_Unknown     -> (Static, t)
 
   | Tac.Tv_Unsupp ->
-    Tac.fail ("lift failed: cannot inspect " ^ Tac.term_to_string t)
+    fail ("lift failed: cannot inspect term: " ^ Tac.term_to_string t)
+      (range_of_term' t) ["(unsupported term)"]
 
 
 let tac_lift (t: Tac.term): Tac.Tac Tac.term =
@@ -349,49 +459,117 @@ let tac_lift (t: Tac.term): Tac.Tac Tac.term =
   // ignore (Tac.recover (fun () -> Tac.tc e.tac_env t'));
   t'
 
-let fst (#a #b: eqtype): (a & b) -> a = fst
+(*** Examples / test cases ***)
+
+// let lemma_nat_something (x: int) (y: int): Lemma (ensures x > y) = admit ()
+
+// [@@Tac.preprocess_with tac_lift]
+// let eg_instantiate_lemma (x y: stream int): stream int =
+//   lemma_nat_something x y;
+//   x + y
 
 
-// do not support local function bindings yet
-[@@Tac.preprocess_with tac_lift]
-let eg_letrecfun (x: int): int =
-  let rec count (x: int): int = if x > 0 then count (x - 1) else 0 in
-  count 0
+// // local function bindings require explicit type annotations
+// [@@Tac.preprocess_with tac_lift]
+// let eg_letrecfun (x: int): int =
+//   let rec count (x: int): int = if x > 0 then count (x - 1) else 0 in
+//   count 0
 
-[@@Tac.preprocess_with tac_lift]
-let eg_letrec (x: stream int): stream int =
-  let rec count = 0 `fby` count + 1 in
-  let y = (0 <: stream int) in
-  // let z: stream int = 0 in
-  // let rec count (i: int): int = count i in
-  (1 + y) + count
+// [@@Tac.preprocess_with tac_lift]
+// let eg_letrec (x: stream int): stream int =
+//   let rec count = 0 `fby` count + 1 in
+//   let y = (0 <: stream int) in
+//   // let z: stream int = 0 in
+//   // let rec count (i: int): int = count i in
+//   (1 + y) + count
 
-[@@Tac.preprocess_with tac_lift]
-let eg_pairs (x: stream int): stream int =
-  0 `fby` fst (x, x)
+// [@@Tac.preprocess_with tac_lift]
+// let eg_pairs (x: stream int): stream int =
+//   0 `fby` fst (x, x)
 
 
-type ctor = | Ctor: x: int -> y: int -> ctor
-[@@Tac.preprocess_with tac_lift]
-let eg_ctor (add: stream int): stream ctor =
-  let rec rcd =
-    let x = 0 `fby` Ctor?.x rcd + add in
-    let y = 0 `fby` Ctor?.y rcd - add in
-    Ctor x y
-  in
-  rcd
+// type ctor = | Ctor: x: int -> y: int -> ctor
+// [@@Tac.preprocess_with tac_lift]
+// let eg_ctor (add: stream int): stream ctor =
+//   let rec rcd =
+//     let x = 0 `fby` Ctor?.x rcd + add in
+//     let y = 0 `fby` Ctor?.y rcd - add in
+//     Ctor x y
+//   in
+//   rcd
 
-[@@Tac.preprocess_with tac_lift]
-let eg_pairsrec (add: stream int): stream (int & int) =
-  let rec xy =
-    // let (x,y) = xy in
-    let x = 0 `fby` fst xy + add in
-    let y = 0 `fby` snd xy - add in
-    (x, y)
-  in
-  xy
+// [@@Tac.preprocess_with tac_lift]
+// let eg_pairsrec (add: stream int): stream (int & int) =
+//   let rec xy =
+//     let x = 0 `fby` fst xy + add in
+//     let y = 0 `fby` snd xy - add in
+//     (x, y)
+//   in
+//   xy
+
+
+// [@@Tac.preprocess_with tac_lift]
+// let eg_let (x: stream int): stream int =
+//   let y = (x + 1, x - 1)
+//   in
+//   let z = fst y in
+//   let rec count (x: int): int = if x > 0 then count (x - 1) else x in
+//   count z
+
+// [@@Tac.preprocess_with tac_lift]
+// let eg_streaming_match (x: stream int): stream int =
+//   let abs =
+//     match x >= 0 with
+//       | true -> x
+//       | false -> -x
+//   in abs
+
+// [@@Tac.preprocess_with tac_lift]
+// let eg_streaming_if (x: stream int): stream int =
+//   let abs =
+//     if x >= 0 then x else -x
+//   in abs
+
+
+// [@@Tac.preprocess_with tac_lift]
+// let eg_static_match (consts: list int) (x: stream int): stream int =
+//   match consts with
+//   | [] -> 0
+//   | c::_ -> c + x
+
+
+(*** Not supported examples ***)
+// mutual recursion not supported:
+
+// [@@Tac.preprocess_with tac_lift]
+// let eg_letrec_mut (x: int): int =
+//   let rec a = x + b
+//       and b = x - a
+//   in a
+
+// streaming matches cannot bind variables:
+
+// [@@Tac.preprocess_with tac_lift]
+// let eg_streaming_match_bind (x: stream (option int)): stream int =
+//   match x with
+//   | Some e -> e
+//   | None -> 0
+
+// [@@Tac.preprocess_with tac_lift]
+// let eg_streaming_letmatch (xy: stream (int & int)): stream int =
+//   let (x, y) = xy in
+//   x + y
+
+// should work, but doesn't:
+// [@@Tac.preprocess_with tac_lift]
+// let eg_streaming_match_bool (x: stream int): stream bool =
+//   match x >= 0 with
+//     | true -> false
+//     | xr -> xr
+
 
 // fails: cannot typecheck record accessors?
+
 // type record = { x: int; y: int; }
 // [@@Tac.preprocess_with tac_lift]
 // let eg_record (add: stream int): stream int =
@@ -401,21 +579,3 @@ let eg_pairsrec (add: stream int): stream (int & int) =
 //     {x; y}
 //   in
 //   rcd
-
-
-[@@Tac.preprocess_with tac_lift]
-let eg_let (x: stream int): stream int =
-  let y = (x + 1, x - 1)
-  in
-  let z = fst y in
-  let rec count (x: int): int = if x > 0 then count (x - 1) else x in
-  // Tac.print "hello";
-  count z
-
-// mutual recursion not supported:
-
-// [@@Tac.preprocess_with lift]
-// let eg_letrec_mut (x: int): int =
-//   let rec a = x + b
-//       and b = x - a
-//   in a
